Added fixes in Client.Encrypt
* aes_encrypt returns the authTag, so don't try to compute it outside the routine

* Store verification key, not signature key, under "aws-crypto-public-key" in
  encryption context.

* Add function to compute StringToByteSeq(Base64.Encode(_)). In the future, the
  Base64 module may offer routines that operate directly on seq<uint8> instead of
  just seq<char>.

* Use ENDFRAME_SEQUENCE_NUMBER constant instead of numeric literal

* Fix spelling mistake in comment

src/extern/dotnet/EncryptionExtern.cs
@@ -222,7 +222,7 @@ namespace Signature {
                 byte[] bytes = SignatureToByteArray(sig[0], sig[1]);
                 if (bytes.Length != x.SignatureLength()) {
                     // Most of the time, a signature of the wrong length can be fixed
-                    // be negating s in the signature relative to the group order.
+                    // by negating s in the signature relative to the group order.
                     bytes = SignatureToByteArray(sig[0], p.N.Subtract(sig[1]));
                     if (bytes.Length != x.SignatureLength()) {
                         // We give up. :(
