src/SDK/MessageBody.dfy
@@ -23,9 +23,9 @@ module MessageBody {
     var n, sequenceNumber := 0, 1;
     while n + frameLength <= |plaintext|
       invariant 0 <= n <= |plaintext|
-      invariant sequenceNumber <= 0xFFFF_FFFF
+      invariant sequenceNumber <= ENDFRAME_SEQUENCE_NUMBER
     {
-      if sequenceNumber == 0xFFFF_FFFF {
+      if sequenceNumber == ENDFRAME_SEQUENCE_NUMBER {
         return Failure("too many frames");
       }
       var plaintextFrame := plaintext[n..n + frameLength];
@@ -39,16 +39,16 @@ module MessageBody {
   }
 
   method EncryptFrame(algorithmSuiteID: AlgorithmSuite.ID, key: seq<uint8>, frameLength: int, messageID: Msg.MessageID,
-                      plaintext: seq<uint8>, sequenceNumber: int, final: bool)
+                      plaintext: seq<uint8>, sequenceNumber: uint32, final: bool)
       returns (res: Result<seq<uint8>>)
     requires |key| == algorithmSuiteID.KeyLength()
-    requires 0 < frameLength && 0 < sequenceNumber <= 0xFFFF_FFFF
+    requires 0 < frameLength && 0 < sequenceNumber <= ENDFRAME_SEQUENCE_NUMBER
     requires |plaintext| < UINT32_LIMIT
-    requires !final ==> |plaintext| == frameLength && sequenceNumber != 0xFFFF_FFFF
+    requires !final ==> |plaintext| == frameLength && sequenceNumber != ENDFRAME_SEQUENCE_NUMBER
     requires final ==> |plaintext| < frameLength
     requires 4 <= algorithmSuiteID.IVLength()
   {
-    var unauthenticatedFrame := if final then UInt32ToSeq(0xFFFF_FFFF) else [];
+    var unauthenticatedFrame := if final then UInt32ToSeq(ENDFRAME_SEQUENCE_NUMBER) else [];
     var seqNumSeq := UInt32ToSeq(sequenceNumber as uint32);
     unauthenticatedFrame := unauthenticatedFrame + seqNumSeq;
 
@@ -63,21 +63,33 @@ module MessageBody {
     var contentAAD := if final then BODY_AAD_CONTENT_FINAL_FRAME else BODY_AAD_CONTENT_REGULAR_FRAME;
     var aad := messageID + contentAAD + seqNumSeq + UInt64ToSeq(|plaintext| as uint64);
 
-    var encryptedContents :- Encrypt(algorithmSuiteID, iv, key, plaintext, aad);
-    unauthenticatedFrame := unauthenticatedFrame + encryptedContents;
+    var pair :- Encrypt(algorithmSuiteID, iv, key, plaintext, aad);
+    var (encryptedContents, authTag) := pair;
+    unauthenticatedFrame := unauthenticatedFrame + encryptedContents + authTag;
 
-    var authTag :- Encrypt(algorithmSuiteID, iv, key, unauthenticatedFrame, aad);
-    return Success(unauthenticatedFrame + authTag);
+    return Success(unauthenticatedFrame);
   }
 
   const BODY_AAD_CONTENT_REGULAR_FRAME := StringToByteSeq("AWSKMSEncryptionClient Frame");
   const BODY_AAD_CONTENT_FINAL_FRAME := StringToByteSeq("AWSKMSEncryptionClient Final Frame");
 
-  method Encrypt(algorithmSuiteID: AlgorithmSuite.ID, iv: seq<uint8>, key: seq<uint8>, plaintext: seq<uint8>, aad: seq<uint8>) returns (res: Result<seq<uint8>>)
+  const ENDFRAME_SEQUENCE_NUMBER: uint32 := 0xFFFF_FFFF
+
+  method Encrypt(algorithmSuiteID: AlgorithmSuite.ID, iv: seq<uint8>, key: seq<uint8>, plaintext: seq<uint8>, aad: seq<uint8>) returns (res: Result<(seq<uint8>,seq<uint8>)>)
     requires |iv| == algorithmSuiteID.IVLength()
     requires |key| == algorithmSuiteID.KeyLength()
+    ensures match res
+      case Success((ciphertext, authTag)) =>
+        |ciphertext| == |plaintext| &&
+        |authTag| == algorithmSuiteID.TagLength()
+      case Failure(_) => true
   {
     var cipher := AlgorithmSuite.Suite[algorithmSuiteID].params;
-    res := AESEncryption.AES.aes_encrypt(cipher, iv, key, plaintext, aad);
+    var bytes :- AESEncryption.AES.aes_encrypt(cipher, iv, key, plaintext, aad);
+    var n := |plaintext|;
+    if |bytes| != n + algorithmSuiteID.TagLength() {
+      return Failure("unexpected AES encryption result");
+    }
+    return Success((bytes[..n], bytes[n..]));
   }
 }
